Switched GhostTokenPtr's model to an association list to help with injectivity

theories/typing/lib/ghostptrtoken/ghostptrtoken.v
@@ -5,14 +5,47 @@ Set Default Proof Using "Type".
 Open Scope nat.
 Implicit Type 𝔄 𝔅: syn_type.
 
+Notation "'[∗' 'list]' ( k , x ) ∈ l , P" := ((big_opL bi_sep (fun _ '(k, x) => P) l))%core
+(at level 200, l at level 10, k, x at level 1, right associativity)
+  : bi_scope.
+
+Notation al_fmap f := (fmap (prod_map id f)).
+
+Notation list_to_gmap := (@list_to_map loc _ (gmap loc _)).
+
+Lemma elem_of_list_to_map_2' {K A M} `{FinMap K M} (l: list (K * A)) i x:
+  ((list_to_map l): M A) !! i = Some x → ∃ r, l ≡ₚ (i, x) :: r /\ ((list_to_map l): M A) = <[i:=x]>(list_to_map r).
+Proof.
+  intros. induction l as [|[i' x'] r]. apply elem_of_list_to_map_2 in H7. apply elem_of_nil in H7. done.
+  destruct (decide (i'=i)) as [->|?].
+  rewrite list_to_map_cons lookup_insert in H7.
+  injection H7 as <-. exists r. split. reflexivity. 
+  rewrite list_to_map_cons. reflexivity.
+  rewrite list_to_map_cons lookup_insert_ne in H7; [|done].
+  destruct (IHr H7) as (r'&perm&ltm).
+  exists ((i', x')::r'). split. rewrite Permutation_swap -perm. done.
+  rewrite 2! list_to_map_cons ltm insert_commute.
+  done. done.
+Qed.
+
 Section token.
+
   Context `{!typeG Σ}.
 
-  Lemma split_mt_token {𝔄} d l' amπ Φ :
-    (l' ↦∗: (λ vl, [S(d') := d] ∃ (aπm: gmap loc (proph 𝔄)),
-      ⌜vl = [] ∧ amπ = mapply aπm⌝ ∗ Φ d' aπm)) ⊣⊢
-    [S(d') := d] ∃(aπm: gmap loc (proph 𝔄)),
-      ⌜amπ = mapply aπm⌝ ∗ l' ↦∗ [] ∗ Φ d' aπm.
+  Global Instance big_sepAL_persistent {K A} (Φ: K → A → iProp Σ) (l: list (K*A)):
+    (∀ k x, Persistent (Φ k x)) → Persistent ([∗ list] (k, x) ∈ l, Φ k x).
+  Proof.
+    intros. apply big_sepL_persistent. intros ?[??]. done.
+  Qed.
+
+
+  Definition alapply {A B K} (fl: list (K*(B → A))) (x: B) := (al_fmap (.$ x) fl).
+
+  Lemma split_mt_token {𝔄} d l' alπ Φ :
+    (l' ↦∗: (λ vl, [S(d') := d] ∃ (aπl: list (loc * (proph 𝔄))),
+      ⌜vl = [] ∧ alπ = alapply aπl⌝ ∗ Φ d' aπl)) ⊣⊢
+    [S(d') := d] ∃(aπl: list (loc * (proph 𝔄))),
+      ⌜alπ = alapply aπl⌝ ∗ l' ↦∗ [] ∗ Φ d' aπl.
   Proof.
     iSplit.
     - iIntros "(%& ↦ & big)". case d=>// ?. iDestruct "big" as (?[->->]) "Φ".
@@ -21,27 +54,25 @@ Section token.
       iExists []. iFrame "↦". iExists _. by iFrame.
   Qed.
 
-  Lemma split_mt_token' {𝔄} l' amπ Φ :
-    (l' ↦∗: (λ vl, ∃(aπm: gmap loc (proph 𝔄)),
-      ⌜vl = [] ∧ amπ = mapply aπm⌝ ∗ Φ aπm)) ⊣⊢
-    ∃(aπm: gmap loc (proph 𝔄)),
-      ⌜amπ = mapply aπm⌝ ∗ l' ↦∗ [] ∗ Φ aπm.
+  Lemma split_mt_token' {𝔄} l' alπ Φ :
+    (l' ↦∗: (λ vl, ∃(aπl: list (loc * (proph 𝔄))),
+      ⌜vl = [] ∧ alπ = alapply aπl⌝ ∗ Φ aπl)) ⊣⊢
+    ∃(aπl: list (loc * (proph 𝔄))),
+      ⌜alπ = alapply aπl⌝ ∗ l' ↦∗ [] ∗ Φ aπl.
   Proof.
     set Φ' := λ _: nat, Φ. have ->: Φ = Φ' 0 by done.
     by apply (split_mt_token (S _)).
   Qed.
 
-  Lemma ty_share_big_sepM {𝔄} (ty: type 𝔄) E aπm d κ tid q :
+  Lemma ty_share_big_sepAL {𝔄} (ty: type 𝔄) E aπl d κ tid q :
     ↑lftN ⊆ E → lft_ctx -∗ κ ⊑ ty_lft ty -∗
-    &{κ} ([∗ map] l ↦ aπ ∈ aπm, l ↦∗: ty.(ty_own) aπ d tid) -∗ q.[κ]
+    &{κ} ([∗ list] (l, aπ) ∈ aπl, l ↦∗: ty.(ty_own) aπ d tid) -∗ q.[κ]
       ={E}=∗ |={E}▷=>^d |={E}=>
-        ([∗ map] l ↦ aπ ∈ aπm, ty.(ty_shr) aπ d κ tid l) ∗ q.[κ].
+        ([∗ list] (l, aπ) ∈ aπl, ty.(ty_shr) aπ d κ tid l) ∗ q.[κ].
   Proof.
-    rewrite big_opM_map_to_list.
-    rewrite big_opM_map_to_list.
     iIntros (?) "#LFT #In Bor κ".
     iMod (bor_big_sepL with "LFT Bor") as "Bors"; [done|].
-    iInduction (map_to_list aπm) as [|] "IH" forall (q)=>/=.
+    iInduction aπl as [|[l x]] "IH" forall (q)=>/=.
     { iApply step_fupdN_full_intro. by iFrame. }
     iDestruct "κ" as "[κ κ₊]". iDestruct "Bors" as "[Bor Bors]".
     iMod (ty_share with "LFT In Bor κ") as "Toshr"; [done|].
@@ -50,19 +81,18 @@ Section token.
     by iIntros "!> [>[$$] >[$$]]".
   Qed.
 
-  Lemma trans_big_sepM_mt_ty_own {𝔄} (ty: type 𝔄) aπm d tid :
-    ([∗ map] l ↦ aπ ∈ aπm, l ↦∗: ty.(ty_own) aπ d tid) ⊣⊢
-    ∃(wll: vec (list val) (length (map_to_list aπm))), ([∗ list] elt ∈ (vzip (vmap (λ x, x.1) (Vector.of_list (map_to_list aπm))) wll), elt.1 ↦∗ elt.2) ∗
-      ([∗ list] aπwl ∈ vzip (vmap (λ x, x.2) (Vector.of_list (map_to_list aπm))) wll, ty.(ty_own) aπwl.1 d tid aπwl.2).
+  Lemma trans_big_sepAL_mt_ty_own {𝔄} (ty: type 𝔄) aπl d tid :
+    ([∗ list] (l, aπ) ∈ aπl, l ↦∗: ty.(ty_own) aπ d tid) ⊣⊢
+    ∃(wll: vec (list val) (length aπl)), ([∗ list] elt ∈ (vzip (vmap (λ x, x.1) (Vector.of_list aπl)) wll), elt.1 ↦∗ elt.2) ∗
+      ([∗ list] aπwl ∈ vzip (vmap (λ x, x.2) (Vector.of_list aπl)) wll, ty.(ty_own) aπwl.1 d tid aπwl.2).
   Proof.
-    rewrite big_opM_map_to_list.
     iSplit.
-    - iIntros "↦owns". iInduction (map_to_list aπm) as [|] "IH"=>/=.
+    - iIntros "↦owns". iInduction aπl as [|[l x]] "IH"=>/=.
       { iExists [#]. iSplit; [done|done]. }
       iDestruct "↦owns" as "[(%& ↦ & ty) ↦owns]".
       iDestruct ("IH" with "↦owns") as (?) "(↦s & tys)".
       iExists (_:::_). iFrame.
-    - iIntros "(%& ↦s & tys)". iInduction (map_to_list aπm) as [|] "IH"; [done|].
+    - iIntros "(%& ↦s & tys)". iInduction aπl as [|[l x]] "IH"; [done|].
       inv_vec wll=>/= ??.
       iDestruct "↦s" as "[↦ ↦s]". iDestruct "tys" as "[ty tys]".
       iSplitL "↦ ty".
@@ -70,17 +100,15 @@ Section token.
       iApply ("IH" with "↦s tys").
   Qed.
 
-  Definition list_to_gmap {A} `{Countable K} : list (K * A) → gmap K A := list_to_map.
-
-  Lemma remove_mapply {A B} `{Countable K} (aπm: gmap K (A → B)):
-    mapply aπm = λ π, list_to_map (prod_map id (.$ π) <$> (map_to_list aπm)).
+  (* Lemma remove_alapply {A B} `{Countable K} (aπl: gmap K (A → B)):
+    alapply aπl = λ π, list_to_map (prod_map id (.$ π) <$> (map_to_list aπl)).
   Proof.
     apply functional_extensionality. intros.
     rewrite list_to_map_fmap. rewrite list_to_map_to_list. exact.
-  Qed.
+  Qed. *)
 
   Lemma zip_to_prod_map{A B C} (f: B → C) (l: list (A * B)):
-    (zip l.*1 (f <$> l.*2)) = (prod_map id f) <$> l.
+    (zip l.*1 (f <$> l.*2)) = al_fmap f l.
   Proof.
     rewrite zip_with_fmap_r. rewrite zip_with_fst_snd.
     congr fmap.
@@ -88,47 +116,42 @@ Section token.
     unfold prod_map. unfold uncurry. unfold Datatypes.uncurry. unfold fst. unfold snd. unfold id. reflexivity.
   Qed.
 
-  Lemma ty_own_proph_big_sepM_mt {𝔄} (ty: type 𝔄) (n: nat) E aπm d tid κ q :
+  Lemma ty_own_proph_big_sepAL_mt {𝔄} (ty: type 𝔄) (n: nat) E aπl d tid κ q :
   ↑lftN ⊆ E → lft_ctx -∗ κ ⊑ ty_lft ty -∗
-  ([∗ map] l ↦ aπ ∈ aπm, l ↦∗: ty.(ty_own) aπ d tid) -∗ q.[κ]
-    ={E}=∗ |={E}▷=>^d |={E}=> ∃ξl q', ⌜mapply aπm ./ ξl⌝ ∗ q':+[ξl] ∗
+  ([∗ list] (l, aπ) ∈ aπl, l ↦∗: ty.(ty_own) aπ d tid) -∗ q.[κ]
+    ={E}=∗ |={E}▷=>^d |={E}=> ∃ξl q', ⌜alapply aπl ./ ξl⌝ ∗ q':+[ξl] ∗
       (q':+[ξl] ={E}=∗
-        ([∗ map] l ↦ aπ ∈ aπm, l ↦∗: ty.(ty_own) aπ d tid) ∗ q.[κ]).
+        ([∗ list] (l, aπ) ∈ aπl, l ↦∗: ty.(ty_own) aπ d tid) ∗ q.[κ]).
   Proof.
-    rewrite {1} trans_big_sepM_mt_ty_own. iIntros (?) "LFT In (%& ↦ & tys) κ".
+    rewrite {1} trans_big_sepAL_mt_ty_own. iIntros (?) "LFT In (%& ↦ & tys) κ".
     iMod (ty_own_proph_big_sepL with "LFT In tys κ") as "Upd"; [done|].
     iApply (step_fupdN_wand with "Upd"). iIntros "!> >(%&%&%& ξl & Totys) !>".
     iExists _, _.
     apply proph_dep_constr with vec_to_list _ _  in H0. rewrite vec_to_list_apply in H0.
     rewrite vec_to_list_map in H0. rewrite vec_to_list_to_vec in H0.
-    apply proph_dep_constr with (λ x, zip ((map_to_list aπm).*1) x) _ _  in H0.
+    apply proph_dep_constr with (λ x, zip (aπl.*1) x) _ _  in H0.
     iSplit. iPureIntro.
-    rewrite remove_mapply.
-    apply proph_dep_constr.
-    unfold compose in H0. unfold lapply in H0.
+    rewrite /alapply.
+    unfold compose in H0. unfold alapply in H0.
     intros π π' eqv. specialize (H0 π π' eqv).
     rewrite 2! zip_to_prod_map in H0. exact H0.
     iIntros "{$ξl}ξl".
     iMod ("Totys" with "ξl") as "[tys $]".
-    rewrite trans_big_sepM_mt_ty_own.
+    rewrite trans_big_sepAL_mt_ty_own.
     iModIntro. iExists _. iFrame.
   Qed.
 
-  Lemma ty_shr_proph_big_sepM {𝔄} (ty: type 𝔄) (n: nat) E aπm d κ tid κ' q :
+  Lemma ty_shr_proph_big_sepAL {𝔄} (ty: type 𝔄) (n: nat) E aπl d κ tid κ' q :
   ↑lftN ⊆ E → lft_ctx -∗ κ' ⊑ κ -∗ κ' ⊑ ty_lft ty -∗
-  ([∗ map] l ↦ aπ ∈ aπm, ty.(ty_shr) aπ d κ tid l) -∗ q.[κ']
-    ={E}▷=∗ |={E}▷=>^d |={E}=> ∃ξl q', ⌜mapply aπm ./ ξl⌝ ∗ q':+[ξl] ∗
+  ([∗ list] (l, aπ) ∈ aπl, ty.(ty_shr) aπ d κ tid l) -∗ q.[κ']
+    ={E}▷=∗ |={E}▷=>^d |={E}=> ∃ξl q', ⌜alapply aπl ./ ξl⌝ ∗ q':+[ξl] ∗
       (q':+[ξl] ={E}=∗ q.[κ']).
   Proof.
     iIntros (?) "#LFT #In #In' tys κ'".
-    rewrite big_opM_map_to_list.
-    setoid_rewrite remove_mapply.
-    iInduction (map_to_list aπm) as [|] "IH" forall (q).
+    unfold alapply.
+    iInduction aπl as [|[l x]] "IH" forall (q) =>/=.
     { iApply step_fupdN_full_intro. iIntros "!>!>!>!>". iExists [], 1%Qp.
-      iFrame "κ'". iSplit.
-      iPureIntro. intros π π' eqv. rewrite 2! fmap_nil. reflexivity.
-      iSplit; [done|].
-      by iIntros. }
+      iFrame "κ'". iSplit. done. iSplit; [done|]. by iIntros. }
     iDestruct "κ'" as "[κ' κ'₊]". iDestruct "tys" as "[ty tys]".
     iMod (ty_shr_proph with "LFT In In' ty κ'") as "Upd"; [done|].
     iMod ("IH" with "tys κ'₊") as "Upd'".
@@ -136,44 +159,45 @@ Section token.
     iIntros "[>(%&%&%& ξl & Toκ') >(%&%&%& ζl & Toκ'₊)] !>".
     iDestruct (proph_tok_combine with "ξl ζl") as (?) "[ξζl Toξζl]".
     iExists _, _. iFrame "ξζl". iSplit.
-    iPureIntro. intros π π' eqv. 
-    rewrite 2! fmap_cons. unfold list_to_gmap. unfold list_to_gmap in H1.
-    rewrite 2! list_to_map_cons. congr insert. 
-    apply H0. intros ξ ξin. apply eqv. apply elem_of_app. left. exact.
-    apply H1. intros ξ ξin. apply eqv. apply elem_of_app. right. exact.  
+    iPureIntro. apply proph_dep_constr2. apply proph_dep_constr. done. done. 
     iIntros "ξζl". iDestruct ("Toξζl" with "ξζl") as "[ξl ζl]".
     iMod ("Toκ'" with "ξl") as "$". by iMod ("Toκ'₊" with "ζl") as "$".
   Qed.
 
+  Definition big_sepAL {K A} (Φ: K → A → iProp Σ) (l: list (K*A)) :=  ([∗ list] (k, x) ∈ l, Φ k x)%I.
+
+  (* Lemma all_share_peristent {𝔄} (ty: type 𝔄) aπl d' κ tid : Persistent (all_share 𝔄 ty aπl d' κ tid).
+  apply big_sepAL_persistent. intros. apply ty_shr_persistent. Qed. *)
+
   (* Rust's GhostPtrToken<T> *)
-  Program Definition ghostptrtoken_ty {𝔄} (ty: type 𝔄) : type (fmapₛ 𝔄) := {|
+  Program Definition ghostptrtoken_ty {𝔄} (ty: type 𝔄) : type (listₛ (locₛ * 𝔄)) := {|
     ty_size := 0;  ty_lfts := ty.(ty_lfts);  ty_E := ty.(ty_E);
-    ty_own amπ d tid vl :=
-      [S(d') := d] ∃(aπm: gmap loc (proph 𝔄)),
-        ⌜vl = [] ∧ amπ = mapply aπm⌝ ∗
-        ▷ ([∗ map] l ↦ aπ ∈ aπm, (l) ↦∗: ty.(ty_own) aπ d' tid) ∗
-        ([∗ map] l ↦ _ ∈ aπm, freeable_sz' ty.(ty_size) l);
-    ty_shr amπ d κ tid l' :=
-      [S(d') := d] ∃(aπm: gmap loc (proph 𝔄)),
-        ⌜amπ = mapply aπm⌝ ∗
-        ▷ [∗ map] l ↦ aπ ∈ aπm, ty.(ty_shr) aπ d' κ tid l;
+    ty_own alπ d tid vl :=
+      [S(d') := d] ∃(aπl: list (loc * (proph 𝔄))),
+        ⌜vl = [] ∧ alπ = alapply aπl⌝ ∗
+        ▷ (big_sepAL (λ l aπ, l ↦∗: ty.(ty_own) aπ d' tid) aπl) ∗
+        (big_sepAL (λ l _, freeable_sz' ty.(ty_size) l) aπl);
+    ty_shr alπ d κ tid l' :=
+      [S(d') := d] ∃(aπl: list (loc * (proph 𝔄))),
+        ⌜alπ = alapply aπl⌝ ∗
+        ▷ (big_sepAL (λ l aπ, ty.(ty_shr) aπ d' κ tid l) aπl);
   |}%I.
   Next Obligation.
     iIntros (???[]??) "token //". by iDestruct "token" as (?[-> _]) "?".
   Qed.
-  Next Obligation.
-    move=> ??[|?][|?]*/=; try (by iIntros); [lia|]. do 11 f_equiv.
+  Next Obligation. unfold big_sepAL.
+    move=> ??[|?][|?]*/=; try (by iIntros); [lia|]. do 12 f_equiv.
     apply ty_own_depth_mono. lia.
   Qed.
-  Next Obligation.
-    move=> ??[|?][|?]*/=; try (by iIntros); [lia|]. do 7 f_equiv.
+  Next Obligation. unfold big_sepAL.
+    move=> ??[|?][|?]*/=; try (by iIntros); [lia|]. do 8 f_equiv.
     apply ty_shr_depth_mono. lia.
   Qed.
-  Next Obligation.
+  Next Obligation. unfold big_sepAL.
     move=> ?????[|?]*; [by iIntros|]. iIntros "#? (%&?& All)".
-    iExists _. iSplit; [done|].
-    rewrite !big_sepM_forall. iIntros "!> **".
-    iApply ty_shr_lft_mono; by [|iApply "All"].
+    iExists _. iSplit; [done|]. iNext.
+    erewrite !big_sepL_forall; [|intros ?[??]; by apply ty_shr_persistent ..]. iIntros (?[??]?).
+    iApply ty_shr_lft_mono; by [|iApply ("All" $! _ (_,_))].
   Qed.
   Next Obligation.
     iIntros (???? d) "*% #LFT In Bor κ". rewrite split_mt_token. case d.
@@ -185,14 +209,14 @@ Section token.
     iMod (bor_sep with "LFT Bor") as "[Bor _]"; [done|].
     iMod (bor_later_tok with "LFT Bor κ") as "Borκ"; [done|].
     iIntros "/=!>!>!>". iMod "Borκ" as "[Bor κ]".
-    iMod (ty_share_big_sepM with "LFT In Bor κ") as "Toshrs"; [done|].
+    iMod (ty_share_big_sepAL with "LFT In Bor κ") as "Toshrs"; [done|].
     iApply (step_fupdN_wand with "Toshrs"). iIntros "!> >[?$] !>".
     iExists _. by iFrame.
   Qed.
   Next Obligation.
     iIntros (????[|?]) "*% LFT In token κ/="; [done|].
     iDestruct "token" as (?[->->]) "(↦tys & †)". iIntros "!>!>!>".
-    iMod (ty_own_proph_big_sepM_mt with "LFT In ↦tys κ") as "Upd"; [done|done|].
+    iMod (ty_own_proph_big_sepAL_mt with "LFT In ↦tys κ") as "Upd"; [done|done|].
     iApply (step_fupdN_wand with "Upd"). iIntros "!> >(%&%&%& ξl & Totys) !>".
     iExists _, _. iSplit; [done|].
     iIntros "{$ξl}ξl". iMod ("Totys" with "ξl") as "[tys $]". iModIntro.
@@ -201,7 +225,7 @@ Section token.
   Next Obligation.
     iIntros (????[|?]) "*%*% LFT In In' token κ'/="; [done|].
     iDestruct "token" as (?->) "tys". iIntros "!>!>!>".
-    iMod (ty_shr_proph_big_sepM with "LFT In In' tys κ'") as "Toκ'"; [done|done|].
+    iMod (ty_shr_proph_big_sepAL with "LFT In In' tys κ'") as "Toκ'"; [done|done|].
     iIntros "!>!>". iApply (step_fupdN_wand with "Toκ'").
     iIntros ">(%&%&%& ξl & Toκ') !>". iExists _, _. iSplit; [done|].
     iIntros "{$ξl}ξl". by iMod ("Toκ'" with "ξl") as "$".
@@ -209,16 +233,16 @@ Section token.
 
   Global Instance vec_ty_ne {𝔄} : NonExpansive (@ghostptrtoken_ty 𝔄).
   Proof.
-    constructor.
+    constructor; rewrite /ghostptrtoken_ty /big_sepAL.
     exact.  
-    unfold ty_lfts. unfold ghostptrtoken_ty. eapply ty_lfts_ne. exact. 
-    unfold ty_E. unfold ghostptrtoken_ty. eapply ty_E_ne. exact.
-    unfold ty_own. unfold ghostptrtoken_ty.
+    unfold ty_lfts. eapply ty_lfts_ne. exact. 
+    unfold ty_E. eapply ty_E_ne. exact.
+    unfold ty_own.
     assert (ty_size x = ty_size y). eapply ty_size_ne. exact.
     rewrite H0.
-    intros ????. do 13 f_equiv. apply ty_own_ne; [done|done|done|done|done].
+    intros ????. do 14 f_equiv. apply ty_own_ne; [done|done|done|done|done].
     unfold ty_shr. unfold ghostptrtoken_ty.
-    intros ?????. do 9 f_equiv.
+    intros ?????. do 10 f_equiv.
     apply ty_shr_ne; [done|done|done|done|done|done].
   Qed.
 End token.
