theories/typing/lib/ghostptrtoken/ghostptrtoken_basic.v
@@ -10,48 +10,47 @@ Section ghostptrtoken_basic.
   Context `{!typeG Σ}.
 
   Lemma real_big_sepM_ty_shr {𝔄 𝔅} (ty: type 𝔄) (f: 𝔄 → 𝔅)
-    aπm (d: nat) κ tid E L F q :
+    aπl (d: nat) κ tid E L F q :
     real E L ty f → ↑lftN ⊆ F → lft_ctx -∗ elctx_interp E -∗ llctx_interp L q -∗
-    ([∗ map] l ↦ aπ ∈ aπm, ty.(ty_shr) aπ d κ tid l)
+    ([∗ list] (l, aπ) ∈ aπl, ty.(ty_shr) aπ d κ tid l)
       ={F}▷=∗ |={F}▷=>^d |={F}=>
-        ⌜∃bm, (fmap f) ∘ mapply aπm = const bm⌝ ∗ llctx_interp L q ∗
-        [∗ map] l ↦ aπ ∈ aπm, ty.(ty_shr) aπ d κ tid l.
+        ⌜∃bm, (al_fmap f) ∘ alapply aπl = const bm⌝ ∗ llctx_interp L q ∗
+        [∗ list] (l, aπ) ∈ aπl, ty.(ty_shr) aπ d κ tid l.
   Proof.
-    setoid_rewrite big_opM_map_to_list.
-    rewrite remove_mapply.
-    iIntros ([_ Rl]?) "#LFT #E L tys". iInduction (map_to_list aπm) as [|] "IH" forall (q)=>/=.
-    { iApply step_fupdN_full_intro. iFrame "L". iPureIntro. unfold compose. rewrite fmap_empty. by exists ∅. }
+    iIntros ([_ Rl]?) "#LFT #E L tys". iInduction aπl as [|[??]] "IH" forall (q)=>/=.
+    { iApply step_fupdN_full_intro. iFrame "L". iPureIntro. unfold compose. by exists []. }
     iDestruct "tys" as "[ty tys]". iDestruct "L" as "[L L₊]".
     iMod (Rl with "LFT E L ty") as "Upd"; [done|].
     iMod ("IH" with "L₊ tys") as "Upd'". iCombine "Upd Upd'" as "Upd". iIntros "!>!>".
     iApply (step_fupdN_wand with "Upd"). iIntros "[>(%Eq &$&$) >(%Eq' &$&$)] !%".
-    move: Eq=> [b Eq]. move: Eq'=> [bm Eq']. exists (<[a.1:=b]>bm).
-    fun_ext=>/= π. rewrite fmap_insert. by move: (equal_f Eq π) (equal_f Eq' π)=>/= <-<-.
+    move: Eq=> [b Eq]. move: Eq'=> [bm Eq']. exists ((l,b) :: bm).
+    fun_ext=>/= π. by move: (equal_f Eq π) (equal_f Eq' π)=>/= <-<-.
   Qed.
 
   Global Instance token_type_contractive 𝔄 : TypeContractive (ghostptrtoken_ty (𝔄:=𝔄)).
   Proof.
+    rewrite /ghostptrtoken_ty /big_sepAL.
     split; [by apply type_lft_morphism_id_like|done| |].
-    - move=>/= > ->*. do 13 (f_contractive || f_equiv). by simpl in *.
-    - intros ?????????????. unfold ty_shr. unfold ghostptrtoken_ty. do 9 (f_contractive || f_equiv). by simpl in *.
+    - move=>/= > ->*. do 14 (f_contractive || f_equiv). by simpl in *.
+    - intros ?????????????. unfold ty_shr. unfold ghostptrtoken_ty. do 10 (f_contractive || f_equiv). by simpl in *.
   Qed.
 
   Global Instance token_send {𝔄} (ty: type 𝔄) : Send ty → Send (ghostptrtoken_ty ty).
-  Proof. move=> ?>/=. by do 13 (f_equiv || move=>?). Qed.
+  Proof. rewrite /ghostptrtoken_ty /big_sepAL. move=> ?>/=. by do 14 (f_equiv || move=>?). Qed.
 
   Global Instance token_sync {𝔄} (ty: type 𝔄) : Sync ty → Sync (ghostptrtoken_ty ty).
-  Proof. move=> ?>/=. by do 9 (f_equiv || move=>?). Qed.
+  Proof. rewrite /ghostptrtoken_ty /big_sepAL. move=> ?>/=. by do 10 (f_equiv || move=>?). Qed.
 
   Lemma token_resolve {𝔄} (ty: type 𝔄) Φ E L :
-    resolve E L ty Φ → resolve E L (ghostptrtoken_ty ty) (mforall Φ).
+    resolve E L ty Φ → resolve E L (ghostptrtoken_ty ty) ((lforall Φ) ∘ (fmap snd)).
   Proof.
     iIntros (????[|]???) "#LFT #PROPH #E L token //=".
+    unfold big_sepAL.
     iDestruct "token" as (?[->->]) "[↦tys _]". iIntros "!>!>!>".
-    rewrite trans_big_sepM_mt_ty_own. iDestruct "↦tys" as (?) "[↦ tys]".
+    rewrite trans_big_sepAL_mt_ty_own. iDestruct "↦tys" as (?) "[↦ tys]".
     iMod (resolve_big_sepL_ty_own with "LFT PROPH E L tys") as "Upd"; [done..|].
     iApply (step_fupdN_wand with "Upd").
     rewrite vec_to_list_map. rewrite vec_to_list_to_vec.
-    setoid_rewrite map_Forall_to_list. setoid_rewrite map_to_list_fmap.
     unfold lapply. setoid_rewrite <- list_fmap_compose. setoid_rewrite lforall_Forall.
     setoid_rewrite Forall_fmap. by iIntros "!> H".
   Qed.
@@ -61,21 +60,21 @@ Section ghostptrtoken_basic.
   Proof. move=> ?. apply resolve_just. Qed.
 
   Lemma token_real {𝔄 𝔅} (ty: type 𝔄) (f: 𝔄 → 𝔅) E L :
-    real E L ty f → real (𝔅:=fmapₛ _) E L (ghostptrtoken_ty ty) (fmap f).
+    real E L ty f → real (𝔅:=listₛ (locₛ*_) ) E L (ghostptrtoken_ty ty) (al_fmap f).
   Proof.
-    move=> Rl. split; iIntros (???[|]) "*% LFT E L token //=".
+    move=> Rl. split; iIntros (???[|]) "*% LFT E L token //="; unfold big_sepAL.
     - iDestruct "token" as (?[->->]) "[↦tys †]". iIntros "!>!>!>".
-      rewrite trans_big_sepM_mt_ty_own. iDestruct "↦tys" as (?) "[↦ tys]".
+      rewrite trans_big_sepAL_mt_ty_own. iDestruct "↦tys" as (?) "[↦ tys]".
       iMod (real_big_sepL_ty_own with "LFT E L tys") as "Upd"; [done..|].
       iApply (step_fupdN_wand with "Upd"). iIntros "!> >(%Eq &$&?) !>".
       iSplit; last first.
       { iExists _. iFrame "†". iSplit; [done|]. iNext.
-        rewrite trans_big_sepM_mt_ty_own. iExists _. iFrame. }
-      iPureIntro. move: Eq=> [bl Eq]. exists (list_to_map(zip (map_to_list aπm).*1 (vec_to_list bl))). fun_ext=>/= π.
+        rewrite trans_big_sepAL_mt_ty_own. iExists _. iFrame. }
+      iPureIntro. move: Eq=> [bl Eq]. exists (zip aπl.*1 (vec_to_list bl)). fun_ext=>/= π.
       move: (equal_f Eq π)=>/= <-.
-      rewrite 3! vec_to_list_map. rewrite vec_to_list_to_vec.
-      rewrite -list_fmap_compose. rewrite zip_to_prod_map. rewrite list_to_map_fmap.
-      unfold mapply. rewrite map_fmap_compose. rewrite list_to_map_to_list. reflexivity.
+      rewrite 3! vec_to_list_map  vec_to_list_to_vec.
+      rewrite -list_fmap_compose zip_to_prod_map /alapply -list_fmap_compose.
+      reflexivity.
     - iDestruct "token" as (?) "[%Bor tys]". iIntros "!>!>!>".
       iMod (real_big_sepM_ty_shr with "LFT E L tys") as "Upd"; [done..|].
       iIntros "!>!>". iApply (step_fupdN_wand with "Upd").
@@ -85,27 +84,25 @@ Section ghostptrtoken_basic.
   Qed.
 
   Lemma token_subtype {𝔄 𝔅} (f: 𝔄 → 𝔅) ty ty' E L :
-    subtype E L ty ty' f → subtype E L (ghostptrtoken_ty ty) (ghostptrtoken_ty ty') (fmap f).
+    subtype E L ty ty' f → subtype E L (ghostptrtoken_ty ty) (ghostptrtoken_ty ty') (al_fmap f).
   Proof.
     iIntros (Sub ?) "L". iDestruct (Sub with "L") as "#Sub". iIntros "!> E".
     iDestruct ("Sub" with "E") as "(%EqSz &?&#Own&#Shr)".
-    have Eq: ∀(aπm: gmap loc (proph 𝔄)), fmap f ∘ mapply aπm = mapply (fmap (f ∘.) aπm).
-    { move=> ?. fun_ext=>/= ?. f_equal. unfold mapply. rewrite -2! map_fmap_compose. reflexivity. }
-    do 2 (iSplit; [done|]). iSplit; iIntros "!>" (?[|]) "* token //=".
+    have Eq: ∀(aπl: list (loc*(proph 𝔄))), al_fmap f ∘ alapply aπl = alapply (al_fmap (f ∘.) aπl).
+    { move=> ?. fun_ext=>/= ?. f_equal. unfold alapply. rewrite -2! list_fmap_compose. reflexivity. }
+    do 2 (iSplit; [done|]). iSplit; iIntros "!>" (?[|]) "* token //="; unfold big_sepAL.
     - iDestruct "token" as (?[->->]) "(↦tys & †)". iExists  _.
-      iSplit; [done|]. rewrite 2! big_opM_fmap. rewrite EqSz.
-      iFrame "†".
-      iNext.
-      iApply (big_sepM_impl with "↦tys").
-      iModIntro. iIntros (???) "↦tys". iDestruct "↦tys" as (?) "(↦&tys)". iExists vl.
-      iFrame. iApply ("Own" with "tys").
+      iSplit; [done|]. rewrite 2! big_opL_fmap EqSz. simpl.
+      iSplitR "†"; [iNext|]; iApply (big_sepL_impl with "[$]");
+      iModIntro; iIntros (?[??]?). simpl. iIntros "(%vl&↦&tys)".
+      iExists _. iFrame. iApply "Own". done. simpl. iIntros. done.
     - iDestruct "token" as (?->) "↦". iExists _. rewrite Eq.
       iSplit; [done|].
-      rewrite big_opM_fmap. iApply (big_sepM_impl with "↦").
-      do 2 iModIntro. iIntros (???) "↦". iApply ("Shr" with "↦").
+      rewrite big_opL_fmap. iApply (big_sepL_impl with "↦").
+      do 2 iModIntro. iIntros (???) "↦". destruct x. simpl. iApply ("Shr" with "↦").
   Qed.
   Lemma token_eqtype {𝔄 𝔅} (f: 𝔄 → 𝔅) g ty ty' E L :
-    eqtype E L ty ty' f g → eqtype E L (ghostptrtoken_ty ty) (ghostptrtoken_ty ty') (fmap f) (fmap g).
+    eqtype E L ty ty' f g → eqtype E L (ghostptrtoken_ty ty) (ghostptrtoken_ty ty') (al_fmap f) (al_fmap g).
   Proof. move=> [??]. split; by apply token_subtype. Qed.
 
   (* Rust's GhostPtrToken::new *)
@@ -116,7 +113,7 @@ Section ghostptrtoken_basic.
       return: ["r"].
 
   Lemma ghostptrtoken_new_type {𝔄} (ty: type 𝔄) :
-    typed_val ghostptrtoken_new (fn(∅) → ghostptrtoken_ty ty) (λ post _, post ∅).
+    typed_val ghostptrtoken_new (fn(∅) → ghostptrtoken_ty ty) (λ post _, post []).
   Proof.
     eapply type_fn; [apply _|]=> _ ???. simpl_subst.
     iIntros (???) "_ #TIME _ _ _ Na L C _ Obs". iMod persistent_time_receipt_0 as "⧖".
@@ -126,11 +123,12 @@ Section ghostptrtoken_basic.
     iApply wp_new; [done..|]. iIntros "!>" (l') "[†' _] ⧖".
     do 3 wp_seq.
     rewrite cctx_interp_singleton.
-    iApply ("C" $! [# #_] -[const ∅] with "Na L [-Obs] Obs"). iSplit; [|done].
+    iApply ("C" $! [# #_] -[const []] with "Na L [-Obs] Obs"). iSplit; [|done].
     iExists _, _. do 2 (iSplit; [done|]). rewrite/= freeable_sz_full split_mt_token'. 
-    iFrame "†". iNext. iExists ∅. iSplit.
-    iPureIntro. apply functional_extensionality. intros. unfold mapply. by rewrite fmap_empty.
-    rewrite heap_mapsto_vec_nil 2! big_opM_empty.
+    iFrame "†". iNext. iExists []. iSplit.
+    iPureIntro. apply functional_extensionality. intros. unfold alapply. done.
+    unfold big_sepAL.
+    rewrite heap_mapsto_vec_nil 2! big_sepL_nil.
     iSplit; [done|done].
   Qed.
 End ghostptrtoken_basic.
