theories/typing/lib/ghostptrtoken/ghostptrtoken_insertremove.v
@@ -17,20 +17,20 @@ Section ghostptrtoken_insertremove.
   (* Rust's GhostPtrToken::insert *)
   Lemma ghostptrtoken_insert_type {𝔄} (ty: type 𝔄) :
     typed_val (ghostptrtoken_insert ty) (fn<α>(∅; &uniq{α} (ghostptrtoken_ty ty), box ty) → ptr)
-      (λ post '-[(am, am'); a], forall ptr, am' = <[ptr:=a]>am → post ptr).
+      (λ post '-[(al, al'); a], forall ptr, al' = (ptr,a)::al → post ptr).
   Proof.
-    eapply type_fn; [apply _|]=> α ??[m[x[]]]. simpl_subst.
-    iIntros (?(mπ & bπ &[]) ?) "#LFT #TIME #PROPH #UNIQ #E Na L C /=(m & x &_) #Obs".
-    rewrite !tctx_hasty_val. iDestruct "m" as ([|dm]) "[_ m]"=>//.
-    case m as [[|m|]|]=>//. iDestruct "m" as "[(%ml & >↦m & [#LftIn uniq]) †m]".
-    case ml as [|[[|m'|]|][]]; try by iDestruct "uniq" as ">[]".
+    eapply type_fn; [apply _|]=> α ??[l[x[]]]. simpl_subst.
+    iIntros (?(lπ & bπ &[]) ?) "#LFT #TIME #PROPH #UNIQ #E Na L C /=(l & x &_) #Obs".
+    rewrite !tctx_hasty_val. iDestruct "l" as ([|dl]) "[_ l]"=>//.
+    case l as [[|l|]|]=>//. iDestruct "l" as "[(%ll & >↦l & [#LftIn uniq]) †l]".
+    case ll as [|[[|l'|]|][]]; try by iDestruct "uniq" as ">[]".
     iDestruct "x" as ([|dx]) "[⧖x x]"=>//. case x as [[|x|]|]=>//=.
     iDestruct "x" as "[x' †x]".
      wp_bind (delete _). rewrite freeable_sz_full.
-    iApply ((wp_delete [ #m'])with "[↦m †m]"); [done| by iFrame|]. 
+    iApply ((wp_delete [ #l'])with "[↦l †l]"); [done| by iFrame|]. 
     iNext. iIntros.
     iDestruct "x'" as (?) "(↦x&x')".
-    case dx as [|dx]=>//=. case vl as [|[[|l|]|][]]=>//=.
+    case dx as [|dx]=>//=. case vl as [|[[|p|]|][]]=>//=.
     iDestruct "x'" as "(x'&†x')".
     iDestruct "uniq" as (du ξi [? Eq2]) "[Vo Bor]".
     move: Eq2. set ξ := PrVar _ ξi=> Eq2.
@@ -38,37 +38,34 @@ Section ghostptrtoken_insertremove.
     iMod (bor_acc with "LFT Bor α") as "[(%&%& ⧖u & Pc & ↦token) ToBor]"; [done|].
     wp_seq. iDestruct (uniq_agree with "Vo Pc") as %[<-<-].
     rewrite split_mt_token. case du as [|du]=>//=.
-    iDestruct "↦token" as (aπm Eq1) "(↦l & ↦tys & †)".
+    iDestruct "↦token" as (aπl Eq1) "(↦l & ↦tys & †)".
     iCombine "⧖u ⧖x" as "#⧖". simpl.
     iMod (uniq_update with "UNIQ Vo Pc") as "[Vo Pc]"; [done|].
+    unfold big_sepAL.
     iMod ("ToBor" with "[↦l ↦tys x' † †x' Pc]") as "[Bor α]".
-    (* assert (aπm !! l = None). remember (aπm !! l) as a. rewrite Heqa. case a in Heqa; [|done]. *)
     { iNext. iExists _, _. rewrite split_mt_token. iFrame "⧖ Pc".
-      iExists (<[l:=bπ]>aπm). iFrame. iSplit; [done|].
+      iExists ((p, bπ)::aπl). iFrame. iSplit; [done|].
       iSplitL "↦tys x'".
-      iNext. rewrite big_opM_insert_delete. iSplitL "x'".
+      iNext. rewrite big_sepL_cons. iSplitL "x'".
       iDestruct "x'" as (?) "(↦&own)". iExists (vl). iFrame. iApply (ty_own_depth_mono with "own"). lia.
-      iApply big_sepM_subseteq. apply delete_subseteq. 
-      iApply (big_sepM_impl with "↦tys"). iModIntro. iIntros (???) "H".
+      iApply (big_sepL_impl with "↦tys"). iModIntro. iIntros (?[??]?) "H".
       iDestruct "H" as (?) "(H1&H2)". iExists vl. iFrame. iApply (ty_own_depth_mono with "H2"). fold max. lia.
-      rewrite big_opM_insert_delete. rewrite freeable_sz_full. iFrame "†x'".
-      iApply (big_sepM_subseteq with "†"). apply delete_subseteq. }
+      rewrite freeable_sz_full. iFrame "†x'". }
     iMod ("ToL" with "α L") as "L".
-    set mπ' := λ π, ((mapply (<[l:= bπ]>aπm) π), π ξ).
-    iApply (type_type +[#m' ◁ &uniq{α} (ghostptrtoken_ty ty); #x ◁ box ptr] -[mπ'; const l]
+    set lπ' := λ π, ((alapply ((p, bπ)::aπl) π), π ξ).
+    iApply (type_type +[#l' ◁ &uniq{α} (ghostptrtoken_ty ty); #x ◁ box ptr] -[lπ'; const p]
     with "[] LFT TIME PROPH UNIQ E Na L C [-] []").
     - iApply type_jump; [solve_typing|solve_extract|solve_typing].
-    - iSplitL "Vo Bor"; [|iSplitL; [|done]]. rewrite (tctx_hasty_val #m').
+    - iSplitL "Vo Bor"; [|iSplitL; [|done]]. rewrite (tctx_hasty_val #l').
       iExists _. iSplit; [done|]. 
       iSplit; [done|]. fold max. iExists _, _. rewrite /uniq_body.
-      rewrite (proof_irrel (@prval_to_inh (fmapₛ 𝔄) (fst ∘ mπ')) (@prval_to_inh (fmapₛ 𝔄)  (fst ∘ mπ))).
-      assert ((fst ∘ mπ') = mapply (<[l:= bπ]>(aπm))). exact.
-      rewrite H1. iFrame. iPureIntro. split; [done|done].
+      rewrite (proof_irrel (@prval_to_inh (listₛ (locₛ * 𝔄)) (fst ∘ lπ')) (@prval_to_inh (listₛ (locₛ * 𝔄))  (fst ∘ lπ))).
+      iFrame. exact.
       rewrite (tctx_hasty_val #x). iExists _. iSplit; [done|].
-      simpl. iFrame. iNext. iExists _. iFrame. iExists l. exact.
+      simpl. iFrame. iNext. iExists _. iFrame. iExists p. done.
     - iApply proph_obs_impl; [|done]=> π.
-      move: (equal_f Eq1 π) (equal_f Eq2 π)=>/=. case (mπ π)=>/= ??->-> Imp Eq.
-      apply Imp. rewrite Eq. rewrite -fmap_insert. exact.
+      move: (equal_f Eq1 π) (equal_f Eq2 π)=>/=. case (lπ π)=>/= ??->-> Ilp Eq.
+      apply Ilp. rewrite Eq. reflexivity.
   Qed.
 
   Definition ghostptrtoken_remove {𝔄} (ty: type 𝔄) : val :=
@@ -76,71 +73,73 @@ Section ghostptrtoken_insertremove.
       delete [ #1; "t"];;
       return: ["ptr"].
 
-  (* Rust's GhostPtrToken::remove *)
+  (* Rust's GhostPtrToken::re,ove *)
   Lemma ghostptrtoken_remove_type {𝔄} (ty: type 𝔄) :
     typed_val (ghostptrtoken_remove ty) (fn<α>(∅; &uniq{α} (ghostptrtoken_ty ty), ptr) → box ty)
-      (λ post '-[(am, am'); l], exists(a: 𝔄), (am !! l = Some a) ∧ ((am' = base.delete l am) → post a)).
+      (λ post '-[(al, al'); p], exists(a: 𝔄), ((list_to_gmap al) !! p = Some a) ∧ ((<[p:=a]>(list_to_gmap al') = (list_to_gmap al)) → post a)).
   Proof.
-    eapply type_fn; [apply _|]=> α ??[m[x[]]]. simpl_subst.
-    iIntros (?(mπ & pπ &[]) ?) "#LFT #TIME #PROPH #UNIQ #E Na L C /=(m & x &_) #Obs".
-    rewrite !tctx_hasty_val. iDestruct "m" as ([|dm]) "[_ m]"=>//.
-    case m as [[|m|]|]=>//. iDestruct "m" as "[(%ml & >↦m & [#LftIn uniq]) †m]".
-    case ml as [|[[|m'|]|][]]; try by iDestruct "uniq" as ">[]".
+    eapply type_fn; [apply _|]=> α ??[l[x[]]]. simpl_subst.
+    iIntros (?(lπ & pπ &[]) ?) "#LFT #TIME #PROPH #UNIQ #E Na L C /=(l & x &_) #Obs".
+    rewrite !tctx_hasty_val. iDestruct "l" as ([|dl]) "[_ l]"=>//.
+    case l as [[|l|]|]=>//. iDestruct "l" as "[(%ll & >↦l & [#LftIn uniq]) †l]".
+    case ll as [|[[|l'|]|][]]; try by iDestruct "uniq" as ">[]".
     iDestruct "x" as ([|dx]) "[⧖x x]"=>//. case x as [[|x|]|]=>//=.
     iDestruct "x" as "[x' †x]".
      wp_bind (delete _). rewrite freeable_sz_full.
-    iApply ((wp_delete [ #m'])with "[↦m †m]"); [done| by iFrame|]. 
+    iApply ((wp_delete [ #l'])with "[↦l †l]"); [done| by iFrame|]. 
     iNext. iIntros.
     iDestruct "x'" as (?) "(↦x&x')".
-    iDestruct "x'" as (l) "(%pπeq& %vleq)".
+    iDestruct "x'" as (p) "(%pπeq& %vleq)".
     iDestruct "uniq" as (du ξi [? Eq2]) "[Vo Bor]".
     move: Eq2. set ξ := PrVar _ ξi=> Eq2.
     iMod (lctx_lft_alive_tok α with "E L") as (?) "(α & L & ToL)"; [solve_typing..|].
     iMod (bor_acc with "LFT Bor α") as "[(%&%& ⧖u & Pc & ↦token) ToBor]"; [done|].
     wp_seq. iDestruct (uniq_agree with "Vo Pc") as %[<-<-].
     rewrite split_mt_token. case du as [|du]=>//=.
-    iDestruct "↦token" as (aπm Eq1) "(↦l & ↦token)".
+    iDestruct "↦token" as (aπl Eq1) "(↦l & ↦token)".
     iCombine "⧖u ⧖x" as "#⧖". simpl.
     iMod (proph_obs_sat with "PROPH Obs") as "%ObsSat"; [done|].
-    destruct ObsSat. rewrite (surjective_pairing_fun mπ) in H1.
-    rewrite Eq1 in H1. rewrite pπeq in H1. simpl in H1.
+    remember ((list_to_gmap aπl) !! p) as bπ. symmetry in Heqbπ. destruct bπ as [bπ|]; last first.
+    destruct ObsSat. rewrite (surjective_pairing_fun lπ) in H1.
+    rewrite Eq1 in H1. rewrite pπeq in H1. simpl in H1. 
     destruct H1 as (?&Contains&?).
-    rewrite lookup_fmap_Some in Contains. destruct Contains as (bπ&?&Contains).
-    rewrite (big_opM_delete _ aπm l); [|done].
-    rewrite (big_opM_delete _ aπm l); [|done].
+    rewrite /alapply list_to_map_fmap lookup_fmap Heqbπ in Contains. done.
+    destruct (elem_of_list_to_map_2' _ _ _ Heqbπ) as (rπ&perm&reinsert).
+    unfold big_sepAL.
+    iEval (rewrite perm 2! big_sepL_cons) in "↦token".
     iDestruct "↦token" as "((↦x' & ↦) & †x' & †)".
     iMod (uniq_update with "UNIQ Vo Pc") as "[Vo Pc]"; [done|].
-    assert ((S du `max` dx) = S(du `max` (pred dx))); [by lia|]. rewrite H3 /=.
+    assert ((S du `max` dx) = S(du `max` (pred dx))); [by lia|]. rewrite H1 /=.
     iMod ("ToBor" with "[↦l ↦ † Pc]") as "[Bor α]".
     { iNext. iExists _, _. rewrite split_mt_token. iFrame "⧖ Pc".
       iExists _. iFrame. iSplit; [done|].
-      iNext. iApply (big_sepM_impl with "↦"). iModIntro. iIntros (???) "H".
+      iNext. iApply (big_sepL_impl with "↦"). iModIntro. iIntros (?[??]?) "H".
       iDestruct "H" as (?) "(H1&H2)". iExists _. iFrame. iApply (ty_own_depth_mono with "H2"). fold max. lia.
     }
     iMod ("ToL" with "α L") as "L".
-    set mπ' := λ π, ((mapply (base.delete l aπm) π), π ξ).
-    iApply (type_type +[#m' ◁ &uniq{α} (ghostptrtoken_ty ty); #x ◁ box (box ty)] -[mπ'; bπ]
+    set lπ' := λ π, ((alapply rπ π), π ξ).
+    iApply (type_type +[#l' ◁ &uniq{α} (ghostptrtoken_ty ty); #x ◁ box (box ty)] -[lπ'; bπ]
     with "[] LFT TIME PROPH UNIQ E Na L C [-] []").
     - iApply type_jump; [solve_typing|solve_extract|solve_typing].
-    - iSplitL "Vo Bor"; [|iSplitL; [|done]]. rewrite (tctx_hasty_val #m').
+    - iSplitL "Vo Bor"; [|iSplitL; [|done]]. rewrite (tctx_hasty_val #l').
       iExists _. iSplit; [done|]. 
       iSplit; [done|]. fold max. iExists _, _. rewrite /uniq_body.
-      rewrite (proof_irrel (@prval_to_inh (fmapₛ 𝔄) (fst ∘ mπ')) (@prval_to_inh (fmapₛ 𝔄)  (fst ∘ mπ))).
-      assert ((fst ∘ mπ') = mapply (base.delete l aπm)). exact.
-      rewrite H4. iFrame. iPureIntro. split; [done|done].
+      rewrite (proof_irrel (@prval_to_inh (listₛ (locₛ * 𝔄)) (fst ∘ lπ')) (@prval_to_inh (listₛ (locₛ * 𝔄)) (fst ∘ lπ))).
+      replace (fst ∘ lπ') with (alapply rπ); [|done].
+      iFrame. iPureIntro. split; [done|done].
       rewrite (tctx_hasty_val #x). iExists _. iSplit; [done|]. rewrite vleq.
       simpl. iFrame. iNext. iExists _. 
       iFrame. simpl. rewrite freeable_sz_full. iFrame. 
       iNext. iDestruct "↦x'" as (?) "(a & rest)". iExists vl0. iFrame.
       iApply ty_own_depth_mono; [|done]. lia.
     - iApply proph_obs_impl; [|done]=> π.
-      move: (equal_f Eq1 π) (equal_f Eq2 π)=>/=. case (mπ π)=>/= ??->-> Imp Eq.
+      move: (equal_f Eq1 π) (equal_f Eq2 π)=>/=. case (lπ π)=>/= ??->-> Imp Eq.
       destruct Imp as (xv&xeq&Imp).
-      rewrite lookup_fmap_Some in xeq. destruct xeq as (xπ&xeq&lookup_eq).
+      rewrite /alapply list_to_map_fmap lookup_fmap_Some in xeq. destruct xeq as (xπ&<-&lookup_eq).
       rewrite (equal_f pπeq)/= in lookup_eq.
-      rewrite lookup_eq in Contains. injection Contains as xeqb.
-      rewrite -xeqb xeq. apply Imp. rewrite Eq.
-      unfold mapply. rewrite fmap_delete. f_equal.
+      rewrite lookup_eq in Heqbπ. injection Heqbπ as ->.
+      apply Imp. rewrite Eq.
+      rewrite /alapply 2! list_to_map_fmap -fmap_insert. f_equal.
       rewrite (equal_f pπeq). exact.
   Qed.
 End ghostptrtoken_insertremove.
